experiment/Experiment.Steel.CondSolver.Test.fst
@@ -1,0 +1,200 @@
+module Experiment.Steel.CondSolver.Test
+
+module M    = Experiment.Steel.Repr.M
+module U    = Learn.Util
+module L    = FStar.List.Pure
+module Ll   = Learn.List
+module Fin  = FStar.Fin
+module Perm = Learn.Permutation
+
+open FStar.Tactics
+open Learn.Tactics.Util
+open Steel.Effect.Common
+open Experiment.Steel.CondSolver
+
+
+unfold
+let specT (a : Type) (pre : M.pre_t) (post : M.post_t a) : M.prog_tree a
+  = M.Tspec a pre post (fun _ -> True) (fun _ _ _ -> True)
+
+let rec repeat_n (n : nat) (t : M.prog_tree unit) : M.prog_tree unit
+  = if n = 0 then M.Tret unit () (fun _ -> [])
+    else M.Tbind unit unit t (fun () -> repeat_n (n-1) t)
+
+let norm_test () : Tac unit
+  = norm [delta_only [`%repeat_n; `%Ll.initi];
+          delta_qualifier ["unfold"];
+          iota; zeta; primops]
+
+
+let test_TCspec_u (v0 v1 : vprop') : squash True =
+  _ by (let post' = fresh_uvar (Some (`(M.post_t int))) in
+        let _ =
+          build (`(M.tree_cond (specT int [(`@v0)] (fun _ -> [(`@v1)]))
+                               [(`@v0)] (`#post')))
+          (fun () -> norm_test (); build_TCspec false)
+        in ())
+
+let test_TCspec_p (v0 v1 v2 : vprop') (vx : int -> vprop')
+  : M.tree_cond (specT int [v0; v1] (fun x -> [v0; vx x]))
+                ([v0; v1; v2]) (fun x -> [v2; vx x; v0])
+  = _ by (norm_test (); let _ = build_TCspec true in ())
+
+
+let test_TCret_u (v0 v1 : vprop') : squash True =
+  _ by (let post' = fresh_uvar (Some (`(M.post_t int))) in
+        let _,_ =
+          build (`(M.tree_cond (M.Tret int 42 (fun _ -> [])) [(`@v0); (`@v1)] (`#post')))
+          (fun () -> build_TCret false)
+        in ())
+
+let test_TCret_p (v0 : vprop') (vx0 vx1 : int -> vprop')
+  : M.tree_cond (M.Tret int 42 (fun _ -> []))
+                ([v0; vx0 42; vx1 42]) (fun x -> [v0; vx1 x; vx0 42])
+  = _ by (let _ = build_TCret true in ())
+
+
+let test_TCbind_u (v0 v1 : vprop') (vx0 : int -> vprop') : squash True =
+  _ by (let post' = fresh_uvar (Some (`(M.post_t int))) in
+        let _,() =
+          build (`(M.tree_cond
+            (M.Tbind int int (specT int []          (fun x -> [(`@vx0) x]))
+                   (fun x -> specT int [(`@vx0) x] (fun _ -> [(`@v1)])))
+            [(`@v0)] (`#post')))
+          (fun () ->
+            norm_test ();
+            apply (`M.TCbind);
+            let _ = build_TCspec false in
+            let x = intro () in
+            norm_cond_sol ();
+            let post1 = fresh_uvar None in
+            apply_raw (`(__defer_post_unification (`#post1)));
+            let _ = build_TCspec false in
+            norm_cond_sol (); trefl ()
+          )
+        in ())
+
+let test_TCbind_p (v0 v1 : vprop') (vx0 vx1 : int -> vprop')
+  : M.tree_cond
+        (M.Tbind int int (specT int []      (fun x -> [vx0 x])    )
+               (fun x -> specT int [vx0 x] (fun y -> [v1; vx1 y])))
+            [v0] (fun y -> [v0; vx1 y; v1])
+  = _ by (
+    norm_test ();
+    apply (`M.TCbind);
+    let _ = build_TCspec false in
+    let x = intro () in
+    norm_cond_sol ();
+    let _ = build_TCspec true in
+    ()
+  )
+
+
+let test_TCbindP_u (v0 v1 : vprop') (vx0 : int -> vprop') (wp : pure_wp int) (f : unit -> PURE int wp) : squash True =
+  _ by (let post' = fresh_uvar (Some (`(M.post_t int))) in
+        let _,() =
+          build (`(M.tree_cond
+            (M.TbindP int int (`@wp) (`@f)
+                    (fun x -> specT int [(`@v0)] (fun y -> [(`@vx0) y])))
+            [(`@v0); (`@v1)] (`#post')))
+          (fun () ->
+            norm_test ();
+            apply (`M.TCbindP);
+            let x = intro () in
+            let post1 = fresh_uvar None in
+            apply_raw (`(__defer_post_unification (`#post1)));
+            let _ = build_TCspec false in
+            norm_cond_sol (); trefl ()
+          )
+        in ())
+
+let test_TCbindP_p (v0 v1 : vprop') (vx0 : int -> vprop') (wp : pure_wp int) (f : unit -> PURE int wp)
+  : M.tree_cond
+        (M.TbindP int int wp f
+                (fun x -> specT int [v0] (fun y -> [vx0 y])))
+            [v0; v1] (fun y -> [v1; vx0 y])
+  = _ by (
+    norm_test ();
+    apply (`M.TCbindP);
+    let x = intro () in
+    let _ = build_TCspec true in ()
+  )
+
+
+let test_build_tree_cond_0 (v0 v1 : vprop') (vx0 vx1 : int -> vprop')
+  : M.tree_cond
+        (M.Tbind int int (specT int []      (fun x -> [vx0 x]))
+               (fun x -> specT int [vx0 x] (fun y -> [v1; vx1 y])))
+            [v0] (fun y -> [v0; vx1 y; v1])
+  = _ by (norm_test (); let shp = build_tree_cond true in _)
+
+let test_build_prog_cond_0 (v0 v1 : vprop') (vx0 vx1 : int -> vprop')
+  : M.prog_cond
+        (M.Tbind int int (specT int []      (fun x -> [vx0 x]))
+               (fun x -> specT int [vx0 x] (fun y -> [v1; vx1 y])))
+        [v0] (fun y -> [v0; vx1 y; v1])
+  = _ by (norm_test (); build_prog_cond ())
+
+let _ = fun v0 v1 vx0 vx1 ->
+  assert (U.print_util (test_build_prog_cond_0 v0 v1 vx0 vx1))
+      by (norm [delta_only [`%test_build_prog_cond_0]; delta_attr [`%__tac_helper__]];
+          dump "print")
+
+(*let test_build_prog_cond_1 (v : int -> vprop')
+  : M.prog_cond
+        (repeat_n 100 (specT unit (Ll.initi 0 2 v) (fun () -> Ll.initi 0 2 (fun i -> v (1 - i)))))
+        (Ll.initi 0 5 v) (fun () -> Ll.initi 0 5 v)
+  = _ by (norm_test ();
+          let t = timer_start "buil_prog_cond" in
+          build_prog_cond ();
+          timer_stop t)*)
+
+
+/// This example fails because the resolution of the innermost [M.Tret] has to infer its post. In this case the
+/// inferred post is simply the current vprops, ignoring the returned value (i.e. [fun _ -> pre] in [__build_TCret_u]).
+/// But at this point pre is [vx0 x] where [x] is bound, the inferred post is thus [fun _ -> [vx0 x]] which
+/// depends on [x].
+[@@expect_failure [228]]
+let test_build_tree_cond__Tret_u_0 (vx0 : int -> vprop')
+  : M.tree_cond
+        (M.Tbind int int
+            (M.Tbind int int (specT int [] (fun x -> [vx0 x])) (fun x -> M.Tret int x (fun _ -> [])))
+            (fun x -> M.Tret int x (fun _ -> [])))
+        [] (fun x -> [vx0 x])
+  = _ by (norm_test (); let _ = build_tree_cond true in ())
+
+/// This example works because the resolution of [M.Tret] is given the expected post (the post of the whole
+/// program), [fun x' -> [vx0 x']].
+let test_build_tree_cond__Tret_u_1 (vx0 : int -> vprop')
+  : M.tree_cond
+        (M.Tbind int int (specT int [] (fun x -> [vx0 x])) (fun x -> M.Tret int x (fun _ -> [])))
+        [] (fun x -> [vx0 x])
+  = _ by (norm_test (); let _ = build_tree_cond true in ())
+
+/// This example works because we annotate the innermost [M.Tret] with an hint.
+let test_build_tree_cond__Tret_u_2 (v0 : vprop') (vx0 : int -> vprop')
+  : M.tree_cond
+        (M.Tbind int int
+            (M.Tbind int int (specT int [] (fun x -> [v0; vx0 x])) (fun x -> M.Tret int x (fun x' -> [vx0 x'])))
+            (fun x -> M.Tret int x (fun _ -> [])))
+        [] (fun x -> [v0; vx0 x])
+  = _ by (norm_test (); let _ = build_tree_cond true in ())
+
+
+/// This example fails because we cannot find a [v0] in the pre.
+[@@expect_failure [228]]
+let test_build_tree_cond__not_found (v0 : vprop')
+  : M.tree_cond
+        (specT int [v0] (fun _ -> []))
+        [] (fun _ -> [])
+  = _ by (norm_test (); let _ = build_tree_cond true in ())
+
+/// This example fails because we obtain [fun _ -> [v0]] as post which is not unifiable with the expected post
+/// [fun _ -> []]
+[@@expect_failure [228]]
+let test_build_tree_cond__post (v0 : vprop')
+  : M.tree_cond
+        (specT int [] (fun _ -> [v0]))
+        [] (fun _ -> [])
+  = _ by (norm_test (); let _ = build_tree_cond true in ())
+
