experiment/Experiment.Steel.CondSolver.fsti
@@ -488,7 +488,7 @@ let _ = assert (U.print_util (cond_sol_to_equiv (test_cond_sol)))
                 norm normal_cond_sol_to_equiv;
                 fail "print")*)
 
-(*** Building [M.tree_cond] *)
+(*** Building [M.prog_cond] *)
 
 /// The front-end tactic is [build_prog_cond], which solves a goal of the form [M.prog_cond t pre post] where
 /// [t], [pre] and [post] are concrete terms (i.e. do not contain uvars).
@@ -524,7 +524,6 @@ let norm_cond_sol () : Tac unit =
   norm normal_cond_solver
 
 [@@ __tac_helper__]
-private
 let __defer_post_unification
       (#a : Type) (#t : M.prog_tree a) (#pre : M.pre_t) (#post0 : M.post_t a)
       (post1 : M.post_t a)
@@ -600,7 +599,6 @@ let rec shape_tree_of_pre (#pre_n : nat) (#post_n : nat) (ps : pre_shape_tree pr
 /// inferred ('_u' (uvar) functions like [__build_TCspec_u]).
 
 [@@ __tac_helper__]
-private
 let __build_TCspec_u
       (#a : Type) (#pre : M.pre_t) (#post : M.post_t a) (#req : M.req_t pre) (#ens : M.ens_t pre a post)
       (#pre' : M.pre_t)
@@ -619,7 +617,6 @@ let __build_TCspec_u
              (fun x -> Perm.id_n (len L.(post x @ frame)))
 
 [@@ __tac_helper__]
-private
 let __build_TCspec_p
       (#a : Type) (#pre : M.pre_t) (#post : M.post_t a) (#req : M.req_t pre) (#ens : M.ens_t pre a post)
       (#pre' : M.pre_t) (#post' : M.post_t a)
@@ -646,9 +643,8 @@ let __build_TCspec_p
 /// do not depend on the returned value).
 /// The default behaviour is obtained with [sl_hint = fun _ -> []].
 /// This hint is ignored if the post-condition is known from the context ([__build_TCret_p]).
-/// See [_test_build_tree_cond__Tret_u_0] for a minimal example where it is needed.
+/// See [test_build_tree_cond__Tret_u_0] for a minimal example where it is needed.
 [@@ __tac_helper__]
-private
 let __build_TCret_u
       (#a : Type) (#x : a) (#sl_hint : M.post_t a)
       (#pre : M.pre_t)
@@ -663,7 +659,6 @@ let __build_TCret_u
             (serialize_perm (cond_sol_to_equiv cs))
 
 [@@ __tac_helper__]
-private
 let __build_TCret_p
       (#a : Type) (#x : a) (#sl_hint : M.post_t a)
       (#pre : M.pre_t) (#post : M.post_t a)
@@ -829,193 +824,3 @@ let build_prog_cond () : Tac unit
           delta_qualifier ["unfold"];
           iota; zeta; primops; simplify];
     exact (`intro_l_True)
-
-
-(*** Test *)
-
-open Steel.Effect.Common
-
-unfold
-let specT (a : Type) (pre : M.pre_t) (post : M.post_t a) : M.prog_tree a
-  = M.Tspec a pre post (fun _ -> True) (fun _ _ _ -> True)
-
-let rec repeat_n (n : nat) (t : M.prog_tree unit) : M.prog_tree unit
-  = if n = 0 then M.Tret unit () (fun _ -> [])
-    else M.Tbind unit unit t (fun () -> repeat_n (n-1) t)
-
-let norm_test () : Tac unit
-  = norm [delta_only [`%repeat_n; `%Ll.initi];
-          delta_qualifier ["unfold"];
-          iota; zeta; primops]
-
-
-let _test_TCspec_u (v0 v1 : vprop') : squash True =
-  _ by (let post' = fresh_uvar (Some (`(M.post_t int))) in
-        let _ =
-          build (`(M.tree_cond (specT int [(`@v0)] (fun _ -> [(`@v1)]))
-                               [(`@v0)] (`#post')))
-          (fun () -> norm_test (); build_TCspec false)
-        in ())
-
-let _test_TCspec_p (v0 v1 v2 : vprop') (vx : int -> vprop')
-  : M.tree_cond (specT int [v0; v1] (fun x -> [v0; vx x]))
-                ([v0; v1; v2]) (fun x -> [v2; vx x; v0])
-  = _ by (norm_test (); let _ = build_TCspec true in ())
-
-
-let _test_TCret_u (v0 v1 : vprop') : squash True =
-  _ by (let post' = fresh_uvar (Some (`(M.post_t int))) in
-        let _,_ =
-          build (`(M.tree_cond (M.Tret int 42 (fun _ -> [])) [(`@v0); (`@v1)] (`#post')))
-          (fun () -> build_TCret false)
-        in ())
-
-let _test_TCret_p (v0 : vprop') (vx0 vx1 : int -> vprop')
-  : M.tree_cond (M.Tret int 42 (fun _ -> []))
-                ([v0; vx0 42; vx1 42]) (fun x -> [v0; vx1 x; vx0 42])
-  = _ by (let _ = build_TCret true in ())
-
-
-let _test_TCbind_u (v0 v1 : vprop') (vx0 : int -> vprop') : squash True =
-  _ by (let post' = fresh_uvar (Some (`(M.post_t int))) in
-        let _,() =
-          build (`(M.tree_cond
-            (M.Tbind int int (specT int []          (fun x -> [(`@vx0) x]))
-                   (fun x -> specT int [(`@vx0) x] (fun _ -> [(`@v1)])))
-            [(`@v0)] (`#post')))
-          (fun () ->
-            norm_test ();
-            apply (`M.TCbind);
-            let _ = build_TCspec false in
-            let x = intro () in
-            norm_cond_sol ();
-            let post1 = fresh_uvar None in
-            apply_raw (`(__defer_post_unification (`#post1)));
-            let _ = build_TCspec false in
-            norm_cond_sol (); trefl ()
-          )
-        in ())
-
-let _test_TCbind_p (v0 v1 : vprop') (vx0 vx1 : int -> vprop')
-  : M.tree_cond
-        (M.Tbind int int (specT int []      (fun x -> [vx0 x])    )
-               (fun x -> specT int [vx0 x] (fun y -> [v1; vx1 y])))
-            [v0] (fun y -> [v0; vx1 y; v1])
-  = _ by (
-    norm_test ();
-    apply (`M.TCbind);
-    let _ = build_TCspec false in
-    let x = intro () in
-    norm_cond_sol ();
-    let _ = build_TCspec true in
-    ()
-  )
-
-
-let _test_TCbindP_u (v0 v1 : vprop') (vx0 : int -> vprop') (wp : pure_wp int) (f : unit -> PURE int wp) : squash True =
-  _ by (let post' = fresh_uvar (Some (`(M.post_t int))) in
-        let _,() =
-          build (`(M.tree_cond
-            (M.TbindP int int (`@wp) (`@f)
-                    (fun x -> specT int [(`@v0)] (fun y -> [(`@vx0) y])))
-            [(`@v0); (`@v1)] (`#post')))
-          (fun () ->
-            norm_test ();
-            apply (`M.TCbindP);
-            let x = intro () in
-            let post1 = fresh_uvar None in
-            apply_raw (`(__defer_post_unification (`#post1)));
-            let _ = build_TCspec false in
-            norm_cond_sol (); trefl ()
-          )
-        in ())
-
-let _test_TCbindP_p (v0 v1 : vprop') (vx0 : int -> vprop') (wp : pure_wp int) (f : unit -> PURE int wp)
-  : M.tree_cond
-        (M.TbindP int int wp f
-                (fun x -> specT int [v0] (fun y -> [vx0 y])))
-            [v0; v1] (fun y -> [v1; vx0 y])
-  = _ by (
-    norm_test ();
-    apply (`M.TCbindP);
-    let x = intro () in
-    let _ = build_TCspec true in ()
-  )
-
-
-let _test_build_tree_cond_0 (v0 v1 : vprop') (vx0 vx1 : int -> vprop')
-  : M.tree_cond
-        (M.Tbind int int (specT int []      (fun x -> [vx0 x]))
-               (fun x -> specT int [vx0 x] (fun y -> [v1; vx1 y])))
-            [v0] (fun y -> [v0; vx1 y; v1])
-  = _ by (norm_test (); let shp = build_tree_cond true in _)
-
-let _test_build_prog_cond_0 (v0 v1 : vprop') (vx0 vx1 : int -> vprop')
-  : M.prog_cond
-        (M.Tbind int int (specT int []      (fun x -> [vx0 x]))
-               (fun x -> specT int [vx0 x] (fun y -> [v1; vx1 y])))
-        [v0] (fun y -> [v0; vx1 y; v1])
-  = _ by (norm_test (); build_prog_cond ())
-
-let _ = fun v0 v1 vx0 vx1 ->
-  assert (U.print_util (_test_build_prog_cond_0 v0 v1 vx0 vx1))
-      by (norm [delta_only [`%_test_build_prog_cond_0]; delta_attr [`%__tac_helper__]];
-          dump "print")
-
-(*let _test_build_prog_cond_1 (v : int -> vprop')
-  : M.prog_cond
-        (repeat_n 100 (specT unit (Ll.initi 0 2 v) (fun () -> Ll.initi 0 2 (fun i -> v (1 - i)))))
-        (Ll.initi 0 5 v) (fun () -> Ll.initi 0 5 v)
-  = _ by (norm_test ();
-          let t = timer_start "buil_prog_cond" in
-          build_prog_cond ();
-          timer_stop t)*)
-
-
-/// This example fails because the resolution of the innermost [M.Tret] has to infer its post. In this case the
-/// inferred post is simply the current vprops, ignoring the returned value (i.e. [fun _ -> pre] in [__build_TCret_u]).
-/// But at this point pre is [vx0 x] where [x] is bound, the inferred post is thus [fun _ -> [vx0 x]] which
-/// depends on [x].
-[@@expect_failure [228]]
-let _test_build_tree_cond__Tret_u_0 (vx0 : int -> vprop')
-  : M.tree_cond
-        (M.Tbind int int
-            (M.Tbind int int (specT int [] (fun x -> [vx0 x])) (fun x -> M.Tret int x (fun _ -> [])))
-            (fun x -> M.Tret int x (fun _ -> [])))
-        [] (fun x -> [vx0 x])
-  = _ by (norm_test (); let _ = build_tree_cond true in ())
-
-/// This example works because the resolution of [M.Tret] is given the expected post (the post of the whole
-/// program), [fun x' -> [vx0 x']].
-let _test_build_tree_cond__Tret_u_1 (vx0 : int -> vprop')
-  : M.tree_cond
-        (M.Tbind int int (specT int [] (fun x -> [vx0 x])) (fun x -> M.Tret int x (fun _ -> [])))
-        [] (fun x -> [vx0 x])
-  = _ by (norm_test (); let _ = build_tree_cond true in ())
-
-/// This example works because we annotate the innermost [M.Tret] with an hint.
-let _test_build_tree_cond__Tret_u_2 (v0 : vprop') (vx0 : int -> vprop')
-  : M.tree_cond
-        (M.Tbind int int
-            (M.Tbind int int (specT int [] (fun x -> [v0; vx0 x])) (fun x -> M.Tret int x (fun x' -> [vx0 x'])))
-            (fun x -> M.Tret int x (fun _ -> [])))
-        [] (fun x -> [v0; vx0 x])
-  = _ by (norm_test (); let _ = build_tree_cond true in ())
-
-
-/// This example fails because we cannot find a [v0] in the pre.
-[@@expect_failure [228]]
-let _test_build_tree_cond__not_found (v0 : vprop')
-  : M.tree_cond
-        (specT int [v0] (fun _ -> []))
-        [] (fun _ -> [])
-  = _ by (norm_test (); let _ = build_tree_cond true in ())
-
-/// This example fails because we obtain [fun _ -> [v0]] as post which is not unifiable with the expected post
-/// [fun _ -> []]
-[@@expect_failure [228]]
-let _test_build_tree_cond__post (v0 : vprop')
-  : M.tree_cond
-        (specT int [] (fun _ -> [v0]))
-        [] (fun _ -> [])
-  = _ by (norm_test (); let _ = build_tree_cond true in ())
