experiment/Experiment.Steel.Repr.Test.Extract.fst
@@ -1,0 +1,7 @@
+module Experiment.Steel.Repr.Test.Extract
+
+module Test = Experiment.Steel.Repr.Test
+
+open Steel.Reference
+
+let test3 (r0 r1 : ref nat) = Test.test3_steel r0 r1
